wip

Matroid/Constructions/ParallelExt.lean
@@ -5,32 +5,58 @@ namespace Matroid
 open Set
 
 variable {α β : Type _}
-
-def parallel_preimage (M : Matroid β) (E : Set α) (f : α → β) : Matroid α := matroid_of_base
-  sorry 
-  sorry
-  sorry 
-  sorry 
-  sorry 
-  sorry 
+ 
 
 
--- def parallel_preimage (M : Matroid β) (E : Set α) (f : α → β) : Matroid α := matroid_of_indep
---   E 
---   ( fun I ↦ M.Indep (f '' I) ∧ InjOn f I ∧ I ⊆ E )
---   ( by simp )
---   ( fun I J ⟨h, h', hE⟩ hIJ ↦ ⟨h.subset (image_subset _ hIJ), InjOn.mono hIJ h', hIJ.trans hE⟩ )
---   ( by
---     rintro I J hI  hImax hJmax
+def parallel_preimage (M : Matroid β) (E : Set α) (f : α → β) : Matroid α := matroid_of_indep
+  E 
+  ( fun I ↦ M.Indep (f '' I) ∧ InjOn f I ∧ I ⊆ E )
+  ( by simp )
+  ( fun I J ⟨h, h', hE⟩ hIJ ↦ ⟨h.subset (image_subset _ hIJ), InjOn.mono hIJ h', hIJ.trans hE⟩ )
+  ( by
+    rintro I J ⟨hI, hIinj, hIE⟩ hImax hJmax
 
---     --
---     -- simp [mem_maximals_iff, iff_true_intro hI, iff_true_intro hIinj, iff_true_intro hIE] at hImax
+    have hI1 : ¬M.Base (f '' I)
+    · refine fun hI' ↦ hImax ⟨⟨hI, hIinj, hIE⟩, fun B ⟨hB, hBinj, hBE⟩ (hB' : _ ⊆ _) x hxB ↦ 
+        hBinj.mem_of_mem_image hB' hxB ?_⟩
+      rw [hI'.eq_of_subset_indep hB (image_subset _ hB')]
+      exact mem_image_of_mem _ hxB
+    simp only [mem_maximals_iff, mem_setOf_eq, and_imp] at hJmax 
+    have' := hI.exists_insert_of_not_basis (J := f '' J) (subset_union_right (f '' J) _) sorry sorry
+    obtain ⟨_, ⟨⟨x,hx,rfl⟩,h'⟩, he'⟩ := this
+    refine' ⟨x, ⟨hx, fun hxI ↦ h' (by exact mem_image_of_mem f hxI)⟩, _, _, _⟩ 
+    · rwa [image_insert_eq]
+    · rw []
+    exact insert_subset (hJmax.1.2.2 hx) hIE
+
+
+
+
+
+    -- have hB1 : M.Base (f '' J)
+    -- · simp only [mem_maximals_iff, mem_setOf_eq, and_imp] at hJmax 
+    --   refine hJmax.1.1.base_of_maximal (fun K hK hss ↦ ?_)
+    --   have := hJmax.2 (y := (f ⁻¹' K) ∩ E) (hK.subset ?_)
+
+    --   rw [hJmax.2 (y := (f ⁻¹' K) ∩ E)]
+      
+      
     
---   )
---   sorry
---   ( fun I h ↦ h.2.2 )
+
+    --
+    -- simp [mem_maximals_iff, iff_true_intro hI, iff_true_intro hIinj, iff_true_intro hIE] at hImax
+    
+  )
+  sorry
+  ( fun I h ↦ h.2.2 )
+
+
 
 @[simp] theorem parallel_preimage_indep_iff {M : Matroid β} {E : Set α} {f : α → β} {I : Set α} : 
     (M.parallel_preimage E f).Indep I ↔ (M.Indep (f '' I) ∧ InjOn f I ∧ I ⊆ E) := by 
   sorry 
+
+@[simp] theorem parallel_preimage_ground_eq {M : Matroid β} {E : Set α} {f : α → β} : 
+    (M.parallel_preimage E f).E = E := rfl 
+  
   
